templates/lockfree/skiplist_v0_insert.v
@@ -4,7 +4,7 @@ From iris.heap_lang.lib Require Import nondet_bool.
 From iris.bi.lib Require Import fractional.
 Set Default Proof Using "All".
 From iris.bi.lib Require Import fractional.
-Require Export skiplist_v0 skiplist_v0_search.
+Require Export skiplist_v0 skiplist_v0_traverse.
 
 Section skiplist_v0_search.
 
@@ -13,9 +13,9 @@ Section skiplist_v0_search.
   
   (* Proofs *)
 
-  Lemma insertOp_spec N γ_s γ_t γ_m γ_td γ_ght r (k: K) γ_sy t_id t0:
+  Lemma insertOp_spec N γ_s γ_t γ_m γ_td γ_ght γ_I γ_fp γ_ks r (k: K) γ_sy t_id t0:
         ⌜k ∈ KS⌝ -∗
-          css_inv N γ_t γ_s γ_m γ_td γ_ght (skiplist_inv r) -∗
+          css_inv N γ_t γ_s γ_m γ_td γ_ght (skiplist_inv γ_I γ_fp γ_ks r) -∗
             □ update_helping_protocol N γ_t γ_s γ_td γ_ght -∗
               thread_vars γ_t γ_ght γ_sy t_id t0 -∗
                 {{{ True }}} 
@@ -32,28 +32,26 @@ Section skiplist_v0_search.
     awp_apply (inContents_spec); try done.
     iInv "HInv" as (M0 T0 s0) "(>CSS & >%Habs0 & >Hist & Help & >Templ)".
     { admit. }
-    iDestruct "Templ" as "(PT & %Trans_M0 & %Trans_s0 & Res)". 
+    iDestruct "Templ" as "(Hglob & Res & %PT0 & %Trans_M0)". 
     iAssert (⌜c ∈ FP s0⌝)%I as %FP_p0.
     { (* interpolation *) admit. }
     rewrite (big_sepS_delete _ (FP s0) c); last by eauto.
-    iDestruct "Res" as "(NodeFull_c & Res_rest)".
-    iDestruct "NodeFull_c" as (mc Ic pcc) "(Node & Node_rest)".
-    iAaccIntro with "Node".
+    iDestruct "Res" as "((Node_c & Node_crest) & Res_rest)".
+    iAaccIntro with "Node_c".
     { iIntros "Node". iModIntro. iFrame "Hpost". 
       iNext; iExists M0, T0, s0.
       iFrame "∗%#". 
       rewrite (big_sepS_delete _ (FP s0) c); last by eauto. 
-      iFrame "Res_rest".
-      iExists mc, Ic, pcc. iFrame. }
-    iIntros (res) "(Node & Hres)". iDestruct "Hres" as %Hres.
+      iFrame "Res_rest". iFrame. }
+    iIntros (res) "(Node_c & Hres)". iDestruct "Hres" as %Hres.
     destruct res.
-    - destruct (decide (k ∈ pcc)) as [Hres' | Hres']; last first.
+    - destruct (decide (k ∈ PC s0 c)) as [Hres' | Hres']; last first.
       { exfalso. apply Hres'. by apply Hres. }
-      assert (∀ s n k, k ∈ keyset (intf s n) → (k ∈ (Cont s n) ↔ k ∈ abs s)) as Hkeyset.
+      assert (∀ s n k, k ∈ keyset (FI s n) → (k ∈ (Cont s n) ↔ k ∈ abs s)) as Hkeyset.
       { admit. }
       iAssert (⌜k ∈ abs s⌝)%I as "%".
       { assert (k ∈ Cont s c) as k_in_c.
-        { unfold Cont. destruct (decide (mark s c)); try done.
+        { unfold Cont. destruct (decide (Mark s c)); try done.
           admit. }
         iPureIntro.
         pose proof Hkeyset s c k k_in_ks_c as Hkeyset.
@@ -66,40 +64,112 @@ Section skiplist_v0_search.
       iNext. iExists M0, T0, s0.
       iFrame "∗%".
       rewrite (big_sepS_delete _ (FP s0) c); last by eauto.
-      iFrame. iExists mc, Ic, pcc.
-      iFrame "∗%". wp_pures.
+      iFrame. wp_pures.
       iModIntro. by iApply "Hpost".
     - iModIntro. iSplitR "Hpost".
       iNext. iExists M0, T0, s0.
       iFrame "∗%".
       rewrite (big_sepS_delete _ (FP s0) c); last by eauto.
-      iFrame. iExists mc, Ic, pcc.
-      iFrame "∗%". wp_pures.
+      iFrame. wp_pures.
       wp_apply createNode_spec; try done.
-      iIntros (e em Ie epc) "(Node_e & k_in_e & k_in_Ie_c)".
+      iIntros (e es) "(Node_e & k_in_Ie_c)".
       wp_pures.
       awp_apply (try_constraint_insert_spec k).
       iInv "HInv" as (M1 T1 s1) "(>CSS & >%Habs1 & >Hist & Help & >Templ)".
       { admit. }
       iAssert (⌜p ∈ FP s1⌝)%I as %FP_p1.
       { admit. }
-      iDestruct "Templ" as "(PT & %Trans_M1 & %Trans_s1 & Res)".
+      iDestruct "Templ" as "(Hglob & Res & %PT1 & %Trans_M1)". 
       rewrite (big_sepS_delete _ (FP s1) p); last by eauto.
-      iDestruct "Res" as "(NodeFull_p & Res_rest)".
-      iDestruct "NodeFull_p" as (mp Ip pcp) "(Node & Node_rest)".
-      iAaccIntro with "Node".
-      { iIntros "Node". admit. }
+      iDestruct "Res" as "((Node_p & Node_prest) & Res_rest)".
+      iAaccIntro with "Node_p".
+      { iIntros "Node_p". iModIntro. iFrame. 
+        iNext; iExists M1, T1, s1.
+        iFrame "∗%#". 
+        rewrite (big_sepS_delete _ (FP s1) p); last by eauto. 
+        iFrame "Res_rest". iFrame. }
       iIntros (succ Ip')"(Node_p & Hif)".
       destruct succ; last first.
       + iModIntro. iSplitR "Hpost".
         iNext. iExists M1, T1, s1.
         iFrame "∗%".
         rewrite (big_sepS_delete _ (FP s1) p); last by eauto.
-        iFrame. iExists mp, Ip, pcp.
+        iFrame.
         iDestruct "Hif" as "(_ & %)". subst Ip'. 
         iFrame "∗%".
         wp_pures. iApply "IH"; try done.
       + 
+        set (s1' := 0).
+        iAssert (⌜c ∈ FP s1 ∖ {[p]}⌝)%I as %FP_c_p.
+        { admit. }
+        rewrite (big_sepS_delete _ (FP s1 ∖ {[p]}) c); last by eauto.
+        iDestruct "Res_rest" as "((Node_c & Node_crest) & Res_rest)".
+        iDestruct "Node_prest" as "(HI_p & Hks_p & %Hpure_p)".
+        iDestruct "Node_crest" as "(HI_c & Hks_c & %Hpure_c)".
+        
+        iAssert (own γ_I (◯ (FI s1 p ⋅ FI s1 c)))%I with "[HI_p HI_c]" as "HI_pc".
+        { admit. }
+        assert (FI s1 p ⋅ FI s1 c = FI s1' p ⋅ FI s1' e ⋅ FI s1' c) as flow_upd.
+        { admit. }
+        iEval (rewrite flow_upd) in "HI_pc".
+        iAssert (own γ_I (◯ FI s1' p) ∗ own γ_I (◯ FI s1' e) ∗ own γ_I (◯ FI s1' c))%I 
+          with "[HI_pc]" as "(HI_p & HI_e & HI_c)".
+        { admit. }
+        
+        iAssert (own γ_ks (◯ prod (keyset (FI s1 p) ∪ keyset (FI s1 c), Cont s1 p ∪ Cont s1 c)))
+          with "[Hks_p Hks_c]" as "Hks_pc".
+        { admit. }
+        
+        assert (keyset (FI s1 p) ∪ keyset (FI s1 c) = 
+                  keyset (FI s1' p) ∪ keyset (FI s1' e) ∪ keyset (FI s1' c)) as Keyset_upd.
+        { admit. }
+        assert (k ∈ keyset (FI s1' e)) as k_in_kse.
+        { admit. }
+        
+        assert (Cont s1 p ∪ Cont s1 c ∪ {[k]} = Cont s1' p ∪ Cont s1' c) as Cont_upd.
+        { admit. }
+        
+        iAssert (own γ_ks (◯ prod (keyset (FI s1 p) ∪ keyset (FI s1 c), Cont s1 p ∪ Cont s1 c ∪ {[k]})))
+          with "[Hks_pc]" as "Hks_pc".
+        { admit. }
+        
+        iAssert (own γ_ks (◯ prod (keyset (FI s1' p), Cont s1' p)) ∗
+                    own γ_ks (◯ prod (keyset (FI s1' e), Cont s1' e)) ∗
+                      own γ_ks (◯ prod (keyset (FI s1' c), Cont s1' c)))%I
+          with "[Hks_pc]" as "(Hks_p & Hks_e & Hks_c)".
+        { admit. }
+        
+        assert (node_inv_pure s1' e) as Hpure_e.
+        { admit. }
+        
+        iDestruct "Hglob" as "(HI & HFP & HKS)".
+        
+        iAssert (own γ_I (● GFI s1'))%I with "[HI]" as "HI".
+        { admit. }
+
+        assert (FP s1' = FP s1 ∪ {[e]}) as FP_s1'.
+        { admit. }
+        assert (abs s1' = abs s1 ∪ {[k]}) as abs_s1'.
+        { admit. }
+
+        iAssert (own γ_fp (● FP s1'))%I with "[HFP]" as "HFP".
+        { admit. }
+        
+        iAssert (own γ_ks (● prod (KS, abs s1')))%I with "[HKS]" as "HKS".
+        { admit. }
+        
+        
+        
+        
+        
+        
+        
+                      
+        
+        
+
+        iDestruct "HI_pc" as "(HI_p & HI_e)". & HI_c)". 
+        
         iModIntro. iSplitR "Hpost".
         { iNext. iExists M1, T1, s1.
           iFrame "∗%". admit. }
