templates/lockfree/skiplist_v0_search.v
@@ -19,9 +19,9 @@ Section skiplist_v0_search.
   Notation iProp := (iProp Σ).
 
   
-  Lemma searchOp_spec N γ_s γ_t γ_m γ_td γ_ght r (k: K) γ_sy t_id t0:
+  Lemma searchOp_spec N γ_s γ_t γ_m γ_td γ_ght γ_I γ_fp γ_ks r (k: K) γ_sy t_id t0:
         ⌜k ∈ KS⌝ -∗
-          css_inv N γ_t γ_s γ_m γ_td γ_ght (skiplist_inv r) -∗
+          css_inv N γ_t γ_s γ_m γ_td γ_ght (skiplist_inv γ_I γ_fp γ_ks r) -∗
             □ update_helping_protocol N γ_t γ_s γ_td γ_ght -∗
               thread_vars γ_t γ_ght γ_sy t_id t0 -∗
                 {{{ True }}} 
@@ -38,64 +38,53 @@ Section skiplist_v0_search.
     awp_apply (inContents_spec); try done.
     iInv "HInv" as (M0 T0 s0) "(>CSS & >%Habs0 & >Hist & Help & >Templ)".
     { admit. }
-    iDestruct "Templ" as "(PT & %Trans_M1 & %Trans_s1 & Res)". 
+    iDestruct "Templ" as "(Hglob & Res & %PT0 & %Trans_M0)". 
     iAssert (⌜c ∈ FP s0⌝)%I as %FP_p0.
     { (* interpolation *) admit. }
     rewrite (big_sepS_delete _ (FP s0) c); last by eauto.
-    iDestruct "Res" as "(NodeFull_c & Res_rest)".
-    iDestruct "NodeFull_c" as (mc Ic pcc) "(Node & Node_rest)".
-    iAaccIntro with "Node".
+    iDestruct "Res" as "((Node_c & Node_crest) & Res_rest)".
+    iAaccIntro with "Node_c".
     { iIntros "Node". iModIntro. iFrame "Hpost". 
       iNext; iExists M0, T0, s0.
       iFrame "∗%#". 
       rewrite (big_sepS_delete _ (FP s0) c); last by eauto. 
-      iFrame "Res_rest".
-      iExists mc, Ic, pcc. iFrame. }
-    iIntros (res) "(Node & Hres)". iDestruct "Hres" as %Hres.
+      iFrame "Res_rest". iFrame. }
+    iIntros (res) "(Node_c & Hres)". iDestruct "Hres" as %Hres.
     iSpecialize ("Hpost" $! res).
 
     iAssert (past_state γ_m t0 s)%I as "#Hpast2". { done. }
     iDestruct "Hpast2" as (t)"(%t0_le_t & #Hist_s)".
     iAssert (⌜t ∈ dom M0⌝)%I as %t_in_M0.
     { admit. }
-
-    rewrite (big_sepS_delete _ (dom M0) t); last by eauto.
-    iDestruct "PT" as "(Tick_t & PT_rest)".
+    apply PT0 in t_in_M0.
     iAssert (⌜M0 !!! t = s⌝)%I as %M0_t_s.
-    { admit. } iEval (rewrite M0_t_s) in "Tick_t". 
-    iDestruct "Tick_t" as "(HI & HKS & Ins_r & Out_r & Mark_r & Hbig_star)".
-    rewrite (big_sepS_delete _ (FP s) c); last by eauto.
-    iDestruct "Hbig_star" as "(Node_local & Hbig_star_rest)".
-    iDestruct "Node_local" as "(HIc & Hksc & Hpurec)".
-    iAssert (⌜pcc = PC s c⌝)%I as %->.
-    { (* interpolation *) admit. }
+    { admit. } rewrite M0_t_s in t_in_M0. 
+    destruct t_in_M0 as [Ins_r [Out_r [Mark_r Hbig_star]]].
+    pose proof Hbig_star c FP_c as H'.
+    assert (PC s c = PC s0 c) as PC_c.
+    { admit. }
+
     iAssert (⌜seq_spec searchOp (Cont s c) (Cont s c) res k⌝)%I as %Seq_spec_c.
-    { iPureIntro. unfold seq_spec. split; try done. destruct res; 
-      unfold Cont; destruct (decide (mark s c)); try done.
+    { iPureIntro. 
+      unfold seq_spec. split; try done. destruct res; 
+      unfold Cont; destruct (decide (Mark s c)); try done; rewrite PC_c.
       - by apply Hres.
       - intros ?. by apply Hres. }
-    iAssert (⌜Cont s c ⊆ keyset (intf s c)⌝)%I as %cc_sub_ksc.
-    { by iDestruct "Hpurec" as "(_ & % & _)". }
+    iAssert (⌜Cont s c ⊆ keyset (FI s c)⌝)%I as %cc_sub_ksc.
+    { iPureIntro. by destruct H' as [? [? _]]. }
     iAssert (⌜seq_spec searchOp (abs s) (abs s) res k⌝)%I as %Seq_spec.
     { iPureIntro. unfold seq_spec. split; try done. destruct res.
-      - assert (k ∈ Cont s c) as H'.
+      - assert (k ∈ Cont s c) as H''.
         { unfold Cont. rewrite decide_False; try done.
+          rewrite PC_c.
           by apply Hres. }
-        assert (Cont s c ⊆ abs s) as H''.
+        assert (Cont s c ⊆ abs s) as H'''.
         { admit. }
-        clear -H' H''; set_solver.
+        clear -H'' H'''; set_solver.
       - (* Need this property from all snapshots *)
-        assert (∀ s n k, k ∈ keyset (intf s n) → (k ∈ (Cont s n) ↔ k ∈ abs s)).
+        assert (∀ s n k, k ∈ keyset (FI s n) → (k ∈ (Cont s n) ↔ k ∈ abs s)).
         { admit. }
         admit. }
-(*        
-    iMod (ghost_update_keyset (γ_ks s) searchOp k (Cont s c) (Cont s c) res 
-      (keyset (intf s c)) (abs s)
-      with "[$HKS $Hksc]") as (C') "(%Seq_spec & HKS & Hksc)".
-    { iPureIntro; repeat (split; try done). }
-    iAssert (⌜C' = abs s⌝)%I as %->.
-    { by destruct Seq_spec as [? _]. }
-*)    
     iAssert (past_lin_witness γ_m searchOp k res t0) as "Witn".
     { unfold past_lin_witness, updater_thread. iExists s.
       iFrame "#". by iPureIntro. }
@@ -103,14 +92,9 @@ Section skiplist_v0_search.
     iModIntro. iSplitR "Hpost"; last first.
     { iApply "Hpost"; try done. } 
     { iNext. iExists M0, T0, s0.
-      iFrame "CSS Hist Help %".
-      iSplitR "Node Node_rest Res_rest".
-      rewrite (big_sepS_delete _ (dom M0) t); last by eauto.
-      iFrame "PT_rest". iEval (rewrite M0_t_s). iFrame "HI HKS".
-      rewrite (big_sepS_delete _ (FP s) c); last by eauto.
-      iFrame"Hbig_star_rest". iFrame.
+      iFrame "∗%".
       rewrite (big_sepS_delete _ (FP s0) c); last by eauto.
-      iFrame "Res_rest". iExists mc, Ic, (PC s c). iFrame. }
+      iFrame "Res_rest". iFrame. }
   Admitted.      
     
 End skiplist_v0_search.
